isabelle: Core refactoring

isabelle/core/CoreKindcheck.thy
@@ -34,14 +34,11 @@ definition array_dims_well_kinded :: "CoreDimension list \<Rightarrow> bool" whe
 
 (* Definition of well-kindedness *)
 fun is_well_kinded :: "CoreTyEnv \<Rightarrow> CoreType \<Rightarrow> bool" where
-  "is_well_kinded env (CoreTy_Name typeName argTypes) =
-    (if typeName |\<in>| TE_TypeVars env then
-      argTypes = []
-    else
-      (case fmlookup (TE_Datatypes env) typeName of
-        Some numTyVars \<Rightarrow> length argTypes = numTyVars
-                          \<and> list_all (is_well_kinded env) argTypes
-      | None \<Rightarrow> False))"
+  "is_well_kinded env (CoreTy_Datatype typeName argTypes) =
+    (case fmlookup (TE_Datatypes env) typeName of
+       Some numTyVars \<Rightarrow> length argTypes = numTyVars
+                         \<and> list_all (is_well_kinded env) argTypes
+     | None \<Rightarrow> False)"
 | "is_well_kinded env CoreTy_Bool = True"
 | "is_well_kinded env (CoreTy_FiniteInt sign bits) = True"
 | "is_well_kinded env CoreTy_MathInt = True"
@@ -49,72 +46,53 @@ fun is_well_kinded :: "CoreTyEnv \<Rightarrow> CoreType \<Rightarrow> bool" wher
 | "is_well_kinded env (CoreTy_Record flds) = list_all (is_well_kinded env) (map snd flds)"
 | "is_well_kinded env (CoreTy_Array elemTy dims) =
     (is_well_kinded env elemTy \<and> array_dims_well_kinded dims)"
-| "is_well_kinded env (CoreTy_Meta _) = True"
+| "is_well_kinded env (CoreTy_Meta n) = (n |\<in>| TE_TypeVars env)"
 
 (* Integer types are always well-kinded *)
 lemma is_integer_type_well_kinded:
   "is_integer_type ty \<Longrightarrow> is_well_kinded env ty"
   by (cases ty) auto
 
-(* List of metavariables is always well-kinded *)
+(* A list of metavariables is well-kinded, provided the metavars are all in scope. *)
 lemma list_all_meta_is_well_kinded:
-  "list_all (is_well_kinded env) (map CoreTy_Meta nums)"
-  by (induction nums) auto
+  assumes "\<forall>n \<in> set nums. n |\<in>| TE_TypeVars env"
+  shows "list_all (is_well_kinded env) (map CoreTy_Meta nums)"
+  using assms by (induction nums) auto
 
 
-(* Adding type variables to the environment preserves well-kindedness,
-   provided the new type variables don't shadow datatype names *)
+(* Adding type variables to the environment preserves well-kindedness. Type variables
+   are nat-keyed and datatypes are string-keyed, so no shadowing is possible. *)
 lemma is_well_kinded_extend_tyvars:
   assumes "is_well_kinded env ty"
-   and "extra |\<inter>| fmdom (TE_Datatypes env) = {||}"
   shows "is_well_kinded (env \<lparr> TE_TypeVars := TE_TypeVars env |\<union>| extra \<rparr>) ty"
 using assms proof (induction ty)
-  case (CoreTy_Name name argTypes)
-  define extEnv where "extEnv = env \<lparr> TE_TypeVars := TE_TypeVars env |\<union>| extra \<rparr>"
-  show ?case proof (cases "name |\<in>| TE_TypeVars env")
-    case True
-    (* name is a type variable in env, so also in extended env *)
-    hence "argTypes = []" using assms(1) CoreTy_Name by simp
-    hence "name |\<in>| TE_TypeVars extEnv"
-      using True extEnv_def by simp
-    thus ?thesis using extEnv_def \<open>argTypes = []\<close> by simp
-  next
-    case False
-    (* name is not a type variable in env, so must be a datatype in env *)
-    then obtain numTyVars where
-      dt_lookup: "fmlookup (TE_Datatypes env) name = Some numTyVars" and
-      len_eq: "length argTypes = numTyVars" and
-      args_wk: "list_all (is_well_kinded env) argTypes"
-      using CoreTy_Name(2) by (auto split: option.splits)
-    (* name is a datatype, so it's not in extra (by the non-shadowing assumption) *)
-    have "name |\<notin>| extra"
-      using assms(2) dt_lookup fmlookup_dom_iff by fastforce
-    (* name is neither in extra, nor in the original env's type variables; therefore it
-       is not in the new env's type variables (by definition of the new env) *)
-    hence name_not_tyvar_in_ext: "name |\<notin>| TE_TypeVars extEnv"
-      using False extEnv_def by simp
-    (* By IH, args are well-kinded in extended env *)
-    have args_wk_ext: "list_all (is_well_kinded extEnv) argTypes"
-      using CoreTy_Name.IH args_wk assms(2) extEnv_def list.pred_mono_strong by auto
-    (* TE_Datatypes is unchanged between env and extEnv *)
-    have "fmlookup (TE_Datatypes extEnv) name = Some numTyVars"
-      using dt_lookup extEnv_def by simp
-    thus ?thesis 
-      using name_not_tyvar_in_ext args_wk_ext extEnv_def len_eq by auto
-  qed
+  case (CoreTy_Datatype name argTypes)
+  then obtain numTyVars where
+    dt_lookup: "fmlookup (TE_Datatypes env) name = Some numTyVars" and
+    len_eq: "length argTypes = numTyVars" and
+    args_wk: "list_all (is_well_kinded env) argTypes"
+    by (auto split: option.splits)
+  have args_wk_ext: "list_all (is_well_kinded (env \<lparr> TE_TypeVars := TE_TypeVars env |\<union>| extra \<rparr>)) argTypes"
+    using CoreTy_Datatype.IH args_wk by (simp add: list_all_iff)
+  thus ?case using dt_lookup len_eq by simp
 next
   case (CoreTy_Record flds)
-  have "list_all (is_well_kinded env) (map snd flds)"
-    using CoreTy_Record.prems(1) by auto
-  thus ?case
-    by (smt (verit, del_insts) CoreTy_Record.IH assms(2) imageE is_well_kinded.simps(6)
-        list.pred_mono_strong list.set_map snds.intros)
+  have "\<And>a b. (a, b) \<in> set flds \<Longrightarrow>
+              is_well_kinded (env \<lparr> TE_TypeVars := TE_TypeVars env |\<union>| extra \<rparr>) b"
+  proof -
+    fix a b assume mem: "(a, b) \<in> set flds"
+    from mem CoreTy_Record.prems have "is_well_kinded env b"
+      by (auto simp: list_all_iff)
+    with CoreTy_Record.IH[OF mem] show "is_well_kinded (env \<lparr> TE_TypeVars := TE_TypeVars env |\<union>| extra \<rparr>) b"
+      by (simp add: snds.intros)
+  qed
+  thus ?case by (auto simp: list_all_iff)
 next
   case (CoreTy_Array elemTy dims)
-  have "is_well_kinded env elemTy"
-    using CoreTy_Array.prems(1) by auto
-  thus ?case
-    using CoreTy_Array.IH CoreTy_Array.prems(1) assms(2) by auto
+  thus ?case by auto
+next
+  case (CoreTy_Meta n)
+  thus ?case by simp
 qed (simp_all)
 
 
@@ -126,11 +104,11 @@ lemma is_well_kinded_cong_env:
     and "TE_Datatypes env' = TE_Datatypes env"
   shows "is_well_kinded env' ty = is_well_kinded env ty"
 using assms proof (induction ty)
-  case (CoreTy_Name name argTypes)
+  case (CoreTy_Datatype name argTypes)
   hence IH: "\<And>x. x \<in> set argTypes \<Longrightarrow> is_well_kinded env' x = is_well_kinded env x" by simp
   hence "list_all (is_well_kinded env') argTypes = list_all (is_well_kinded env) argTypes"
     by (induction argTypes) auto
-  then show ?case using CoreTy_Name.prems by (auto split: option.splits)
+  then show ?case using CoreTy_Datatype.prems by (auto split: option.splits)
 next
   case (CoreTy_Record flds)
   hence IH: "\<And>x. x \<in> snd ` set flds \<Longrightarrow> is_well_kinded env' x = is_well_kinded env x" by auto
@@ -174,24 +152,16 @@ lemma apply_subst_preserves_well_kinded:
     and "metasubst_well_kinded env subst"
   shows "is_well_kinded env (apply_subst subst ty)"
 using assms proof (induction ty)
-  case (CoreTy_Name name tyargs)
-  show ?case
-  proof (cases "name |\<in>| TE_TypeVars env")
-    case True
-    hence "tyargs = []" using CoreTy_Name.prems(1) by simp
-    thus ?thesis using True by auto
-  next
-    case False
-    then obtain numTyVars where
-      dt_lookup: "fmlookup (TE_Datatypes env) name = Some numTyVars" and
-      len_eq: "length tyargs = numTyVars" and
-      args_wk: "list_all (is_well_kinded env) tyargs"
-      using CoreTy_Name.prems(1) by (auto split: option.splits)
-    have "list_all (is_well_kinded env) (map (apply_subst subst) tyargs)"
-      using CoreTy_Name.IH args_wk CoreTy_Name.prems(2)
-      by (simp add: list_all_iff)
-    thus ?thesis using False dt_lookup len_eq by simp
-  qed
+  case (CoreTy_Datatype name tyargs)
+  then obtain numTyVars where
+    dt_lookup: "fmlookup (TE_Datatypes env) name = Some numTyVars" and
+    len_eq: "length tyargs = numTyVars" and
+    args_wk: "list_all (is_well_kinded env) tyargs"
+    by (auto split: option.splits)
+  have "list_all (is_well_kinded env) (map (apply_subst subst) tyargs)"
+    using CoreTy_Datatype.IH args_wk CoreTy_Datatype.prems(2)
+    by (simp add: list_all_iff)
+  thus ?case using dt_lookup len_eq by simp
 next
   case (CoreTy_Record flds)
   have "list_all (is_well_kinded env) (map snd flds)"
@@ -208,7 +178,9 @@ next
   show ?case
   proof (cases "fmlookup subst n")
     case None
-    thus ?thesis by simp
+    (* substitution doesn't touch n, so the result is still CoreTy_Meta n,
+       which is well-kinded because n |\<in>| TE_TypeVars env by the input assumption *)
+    thus ?thesis using CoreTy_Meta.prems(1) by simp
   next
     case (Some ty)
     hence "is_well_kinded env ty"
